proof_of_soundness/Theorems.v
@@ -61,6 +61,15 @@ Proof.
 Qed.
 
 
+(* An expressions evaluates to the same value under an expanded
+   function definition list *)
+Theorem evaluation_eq_under_expanded_func_list :
+  forall S E F M e v S' F',
+  exprevalR S E F M e v S' = exprevalR S E F' M e v S'.
+Proof.
+Admitted.
+
+
 Theorem macro_transformation_sound :
   forall (S S': state) (E : environment)
          (F F': func_definitions) (M M': macro_definitions)
@@ -71,48 +80,83 @@ Theorem macro_transformation_sound :
   has_side_effects mexpr = false ->
   get_dynamic_vars mexpr = nil ->
   exprevalR S E F M mexpr v S' ->
-  exprevalR S E F' M' mexpr v S' ->
   e = CallOrInvocation mname ->
   (F', M', e') = transform_macros F M e ->
   exprevalR S E F M e v S' <-> exprevalR S E F' M' e' v S'.
 Proof.
-  intros. unfold transform_macros in H6.
-  rewrite H5,H,H0,H1,H2 in H6. simpl in H6.
-  inversion H6.
+  intros. unfold transform_macros in H5.
+  rewrite H4, H, H0, H1, H2 in H5. simpl in H5.
+  inversion H5.
   split.
   - intros.
      + apply E_FunctionCall with (fstmt:=Skip) (fexpr:=mexpr) (S':=S).
       * unfold definition. simpl.
         rewrite eqb_refl. simpl. reflexivity.
       * apply E_Skip.
-      * rewrite <- H8. rewrite <- H9. apply H4.
-  - intros. rewrite H5. apply E_MacroInvocation with (mexpr := mexpr).
+      * rewrite evaluation_eq_under_expanded_func_list with (F':=F).
+        apply H3.
+  - intros. rewrite H4. apply E_MacroInvocation with (mexpr := mexpr).
     + apply H0.
     + apply H3.
 Qed.
+
+Theorem foo: forall F M e e' F' M',
+  transform_macros F M e = (F', M', e') ->
+  transform_macros F M (ParenExpr e) = (F', M', ParenExpr e').
+Proof.
+  intros. unfold transform_macros.
+Admitted.
+
+Theorem bar: forall F M e e' F' M' F'' M'',
+  transform_macros F M (ParenExpr e) = (F', M', ParenExpr e') ->
+  transform_macros F M e = (F'', M'', e') ->
+  (F', M') = (F'', M'').
+Proof.
+  intros. simpl in H. rewrite H0 in H.
+  inversion H.
+  reflexivity.
+Qed.
+
+Theorem lookup_eq :
+  forall S E F M x F' M' S' v0 v1,
+  exprevalR S E F M (X x) v0 S' ->
+  exprevalR S E F' M' (X x) v1 S' ->
+  v0 = v1.
+Proof.
+Admitted.
+
+Theorem paren_no_paren_eq :
+  forall S E F M pe0 pe1  S' pv0 pv1,
+  exprevalR S E F M pe0 pv0 S' ->
+  exprevalR S E F M pe1 pv1 S' ->
+  pv0 = pv1.
+Proof.
+  intros.
+Admitted.
 
 
 Theorem macro_transformation_sound_all :
   forall (S S': state) (E : environment)
          (F F': func_definitions) (M M': macro_definitions)
          (e e' e'' mexpr: expr) (mname fname: string)
-         (v : Z),
-  definition mname F = None ->
-  invocation mname M = Some mexpr ->
-  has_side_effects mexpr = false ->
-  get_dynamic_vars mexpr = nil ->
-  (F', M', e') = transform_macros F M e ->
-  exprevalR S E F M mexpr v S' ->
-  exprevalR S E F' M' mexpr v S' ->
-  exprevalR S E F M e v S' ->
-  transform_macros F M (ParenExpr e'') = (F', M', e') ->
-  exprevalR S E F' M' e' v S'.
+         (v0 v1 : Z),
+  transform_macros F M e = (F', M', e') ->
+  exprevalR S E F M e v0 S' ->
+  exprevalR S E F' M' e' v1 S' ->
+  v0 = v1.
 Proof.
   intros. induction e.
-  - inversion H3. apply H6.
-  - inversion H3. apply H6.
-  - Abort.
-
+  - inversion H. inversion H0. rewrite <- H9.
+    inversion H. rewrite <- H5 in H1. inversion H1.
+    reflexivity.
+  - inversion H. rewrite <- H5 in H1.
+    eapply lookup_eq.
+    + apply H0.
+    + apply H1.
+  - eapply bar in H.
+    + inversion H. apply IHe.
+      * rewrite H3. rewrite H4.
+Admitted.
 
 
 (* NOTE: May want to note in paper that we have to transform
